Do some preliminary work in parameterizing over StringLike

src/Parsers/SplitterFromParserADT.v
@@ -12,6 +12,7 @@ Require Import Fiat.ADTRefinement.Core.
 Require Import Fiat.Common Fiat.Common.Equality.
 Require Import Fiat.Common.BoundedLookup.
 Require Import Fiat.Common.IterateBoundedIndex.
+Require Import Fiat.Common.StringOperations.
 Require Import Fiat.ADTNotation.BuildComputationalADT.
 
 Set Implicit Arguments.
@@ -128,12 +129,18 @@ Section parser.
   Local Notation mcall2 proj s := (fun n n' st => proj (callcADTMethod (projT1 splitter_impl) (fun idx => ibound (indexb idx))
                                                   (@Build_BoundedIndex _ _ (MethodNames (string_rep Ascii.ascii)) s _ ) st n n')) (only parsing).
 
+  Local Notation ccall0 proj s :=
+    (fun st => proj ((callcADTConstructor (projT1 splitter_impl) (fun idx => ibound (indexb idx))
+                                          (@Build_BoundedIndex _ _ (ConstructorNames (string_rep Ascii.ascii)) s _ )) st))
+      (only parsing).
+
   Local Notation mcall01 s := (mcall0 (fun x => x) s) (only parsing).
   Local Notation mcall02 s := (mcall0 snd s) (only parsing).
   Local Notation mcall11 s := (mcall1 (fun x => x) s) (only parsing).
   Local Notation mcall12 s := (mcall1 snd s) (only parsing).
   Local Notation mcall21 s := (mcall2 (fun x => x) s) (only parsing).
   Local Notation mcall22 s := (mcall2 snd s) (only parsing).
+  Local Notation ccall01 s := (ccall0 (fun x => x) s) (only parsing).
 
   Definition mto_string := Eval simpl in mcall02 "to_string".
   Definition mis_char := Eval simpl in mcall12 "is_char".
@@ -141,6 +148,7 @@ Section parser.
   Definition mlength := Eval simpl in mcall02 "length".
   Definition mtake := Eval simpl in mcall11 "take".
   Definition mdrop := Eval simpl in mcall11 "drop".
+  Definition cnew := Eval simpl in ccall01 "new".
 
   Definition premsplits :=
     Eval simpl in (callcADTMethod
@@ -207,14 +215,19 @@ Section parser.
 
   Ltac prove_string_AbsR :=
     match goal with
-      |- _ ≃ ?z _ _ => unfold z;
-        match goal with
-          H : ?str ≃ ?st
-          |- _ ≃ callcADTMethod (projT1 ?splitter_impl) ?proj ?idx ?st ?arg =>
-          destruct_twice_faster (cMethods_AbsR splitter_impl (proj idx) _ _ H arg);
-            simpl Methods in *;
-            computes_to_inv; subst; eauto
-        end
+      | [ |- _ ≃ ?z _ _ ] => unfold z
+      | [ |- _ ≃ ?z _ ] => unfold z
+    end;
+    match goal with
+      | [ H : ?str ≃ ?st
+          |- _ ≃ callcADTMethod (projT1 ?splitter_impl) ?proj ?idx ?st ?arg ]
+        => destruct_twice_faster (cMethods_AbsR splitter_impl (proj idx) _ _ H arg);
+          simpl Methods in *;
+          computes_to_inv; subst; eauto
+      | [ |- _ ≃ callcADTConstructor (projT1 ?splitter_impl) ?proj ?idx ?arg ]
+        => destruct_twice_faster (cConstructors_AbsR splitter_impl (proj idx) arg);
+          simpl Constructors in *;
+          computes_to_inv; subst; eauto
     end.
 
   Definition mtake_R {arg st str} (H : AbsR (projT2 splitter_impl) str st)
@@ -225,22 +238,28 @@ Section parser.
   : AbsR (projT2 splitter_impl) (drop arg str) (mdrop arg st).
   Proof. prove_string_AbsR. Qed.
 
+  Definition cnew_R {str}
+  : AbsR (projT2 splitter_impl) str (cnew str).
+  Proof. prove_string_AbsR. Qed.
+
   Local Ltac handle_rep0 :=
     repeat intro; cbv beta;
     repeat match goal with
            | [ st : { r : cRep (projT1 splitter_impl) | exists orig, AbsR (projT2 splitter_impl) orig r }%type |- exists orig, AbsR (projT2 splitter_impl) orig (cMethods ?impl _ _ ?arg) ]
              => let H := fresh in
                 destruct st as [? [? H] ];
-                  eexists; first [eapply (mtake_R H)
+                  eexists; first [ eapply (mtake_R H)
                                  | eapply (mdrop_R H) ]
+           | [ |- exists orig, AbsR (projT2 splitter_impl) orig (cConstructors ?impl _ ?arg) ]
+             => eexists; eapply cnew_R
            | [ |- exists orig, AbsR (projT2 splitter_impl) orig (?f _ _ _ _)  ]
-             => unfold f, callcADTMethod
+             => unfold f, callcADTMethod, callcADTConstructor
            | [ |- exists orig, AbsR (projT2 splitter_impl) orig (?f _ _ _)  ]
-             => unfold f, callcADTMethod
+             => unfold f, callcADTMethod, callcADTConstructor
            | [ |- exists orig, AbsR (projT2 splitter_impl) orig (?f _ _)  ]
-             => unfold f, callcADTMethod
+             => unfold f, callcADTMethod, callcADTConstructor
            | [ |- exists orig, AbsR (projT2 splitter_impl) orig (?f _)  ]
-             => unfold f, callcADTMethod
+             => unfold f, callcADTMethod, callcADTConstructor
            end.
 
   Local Obligation Tactic := handle_rep0.
@@ -266,7 +285,7 @@ Section parser.
   Create HintDb parser_adt_method_db discriminated.
   (** We would like to just do
 <<
-  Hint Resolve @mtake_R @mdrop_R : parser_adt_method_db.
+  Hint Resolve @mtake_R @mdrop_R @cnew_R : parser_adt_method_db.
 >>
 
   But [Hint Resolve] only resolves on the head symbol, so this will
@@ -275,12 +294,13 @@ Section parser.
   Extern] for matching.  The latter is about 3x faster (0.015s vs
   0.047s), so we use that one, rather than
 <<
-  Hint Resolve @mtake_R @mdrop_R : parser_adt_method_db.
-  Local Opaque mtake mdrop.
+  Hint Resolve @mtake_R @mdrop_R @cnew_R : parser_adt_method_db.
+  Local Opaque mtake mdrop cnew.
 >>
    *)
   Hint Extern 1 (_ ≃ mtake _ _) => apply @mtake_R : parser_adt_method_db.
   Hint Extern 1 (_ ≃ mdrop _ _) => apply @mdrop_R : parser_adt_method_db.
+  Hint Extern 1 (_ ≃ cnew _) => apply @cnew_R : parser_adt_method_db.
 
   Local Ltac match_erewrite_by match_term lem tac :=
     idtac;
@@ -328,33 +348,39 @@ Section parser.
 
   Local Program Instance adt_based_StringLikeProperties : @StringLikeProperties Ascii.ascii adt_based_StringLike
     := { bool_eq_Equivalence := {| Equivalence_Reflexive := _ |} }.
-  Next Obligation. handle_rep; t @singleton_unique. Qed.
+  Next Obligation. t @singleton_unique. Qed.
   Next Obligation.
-  Proof. handle_rep.
+  Proof.
     let H := fresh in
     t'' H (@singleton_exists);
       edestruct H; try (eexists; erewrite mis_char_eq); intuition eauto.
   Qed.
-  Next Obligation. handle_rep; t @get_0. Qed.
-  Next Obligation. handle_rep; t @get_S. Qed.
-  Next Obligation. handle_rep; t @length_singleton. Qed.
-  Next Obligation. handle_rep; t @bool_eq_char. Qed.
-  Next Obligation. handle_rep; t @is_char_Proper. Qed.
-  Next Obligation. handle_rep; t @length_Proper. Qed.
-  Next Obligation. handle_rep; t @take_Proper. Qed.
-  Next Obligation. handle_rep; t @drop_Proper. Qed.
-  Next Obligation. handle_rep; t @bool_eq_Equivalence. Qed.
-  Next Obligation. handle_rep; t @bool_eq_Equivalence. Qed.
-  Next Obligation. handle_rep; t (fun x y z => @Equivalence_Transitive _ _ (@bool_eq_Equivalence x y z)). Qed.
-  Next Obligation. handle_rep; t @bool_eq_empty. Qed.
-  Next Obligation. handle_rep; t @take_short_length. Qed.
-  Next Obligation. handle_rep; t @take_long. Qed.
-  Next Obligation. handle_rep; t @take_take. Qed.
-  Next Obligation. handle_rep; t @drop_length. Qed.
-  Next Obligation. handle_rep; t @drop_0. Qed.
-  Next Obligation. handle_rep; t @drop_drop. Qed.
-  Next Obligation. handle_rep; t @drop_take. Qed.
-  Next Obligation. handle_rep; t @take_drop. Qed.
+  Next Obligation. t @get_0. Qed.
+  Next Obligation. t @get_S. Qed.
+  Next Obligation. t @length_singleton. Qed.
+  Next Obligation. t @bool_eq_char. Qed.
+  Next Obligation. t @is_char_Proper. Qed.
+  Next Obligation. t @length_Proper. Qed.
+  Next Obligation. t @take_Proper. Qed.
+  Next Obligation. t @drop_Proper. Qed.
+  Next Obligation. t @bool_eq_Equivalence. Qed.
+  Next Obligation. t @bool_eq_Equivalence. Qed.
+  Next Obligation. t (fun x y z => @Equivalence_Transitive _ _ (@bool_eq_Equivalence x y z)). Qed.
+  Next Obligation. t @bool_eq_empty. Qed.
+  Next Obligation. t @take_short_length. Qed.
+  Next Obligation. t @take_long. Qed.
+  Next Obligation. t @take_take. Qed.
+  Next Obligation. t @drop_length. Qed.
+  Next Obligation. t @drop_0. Qed.
+  Next Obligation. t @drop_drop. Qed.
+  Next Obligation. t @drop_take. Qed.
+  Next Obligation. t @take_drop. Qed.
+  Next Obligation.
+  Proof.
+    let H := fresh in
+    t'' H (@bool_eq_from_get);
+      apply H; intro; erewrite <- !mget_eq by eassumption; trivial.
+  Qed.
 
   Definition splits :=
     ibound (indexb (@Build_BoundedIndex _ _ (MethodNames (string_rep Ascii.ascii)) "splits" _ )).
@@ -408,10 +434,9 @@ Section parser.
                              Ascii.ascii adt_based_StringLike string_stringlike G
                              (fun s1 s2 => AbsR (projT2 splitter_impl) s2 (` s1))
                              H0'' _ _ _ H1' p1));
-          apply H; clear H p0 p1; try assumption; simpl
+          apply H; clear H p0 p1; try assumption
     end; [ split | | ];
     handle_rep; eauto with parser_adt_method_db.
-    exact (@mdrop_R n _ _ a).
   Qed.
 
   Definition adt_based_splitter : Splitter G
